Clap/Lang/FB/FB.lean
@@ -49,8 +49,6 @@ def matchesUnaryFunction
     (function a).eval varStore =
     (FB.ofBool p (spec_function (a.toBool varStore))).eval varStore
 
--- def matchesConstraints (p : ℕ) [Fact (p ≥ 2)] (constraints: Prop) (function : Edsl.CircuitStateM p Unit) : Prop :=
-
 lemma right_inv
   {p : ℕ}
   {varStore : ℕ → Option (ZMod p)}
